WIP bumped adequacy, and proved the preservation of fairness

fairneris/adequacy.v
@@ -1,3 +1,4 @@
+From Paco Require Import pacotac.
 From stdpp Require Import finite.
 From trillium Require Import adequacy.
 From fairneris Require Import fairness model_draft.
@@ -28,7 +29,7 @@ Definition always_holds {Σ}
 Definition valid_state_evolution_fairness
            (extr : execution_trace aneris_lang)
            (auxtr : auxiliary_trace (fair_model_to_model simple_fair_model)) :=
-  labels_match extr auxtr ∧ trace_steps simple_trans auxtr.
+  labels_match_trace extr auxtr ∧ trace_steps simple_trans auxtr.
 
 Lemma rel_finitary_valid_state_evolution_fairness :
   rel_finitary valid_state_evolution_fairness.
@@ -38,6 +39,186 @@ Proof. Admitted.
 Lemma gset_union_difference_intersection_L `{Countable A} (X Y : gset A) :
   X = (X ∖ Y) ∪ (X ∩ Y).
 Proof. rewrite union_intersection_l_L difference_union_L. set_solver. Qed.
+
+Theorem strong_simulation_adequacy_multiple Σ
+    `{!anerisPreG (fair_model_to_model simple_fair_model) Σ}
+    (s : stuckness) (es : list aneris_expr) (σ : state) (st : simple_state)
+    A obs_send_sas obs_rec_sas IPs ip lbls :
+  length es ≥ 1 →
+  state_ms σ = mABn (state_get_n st) →
+  (∃ shA shB : socket_handle,
+      state_sockets σ =
+      {[ipA := {[shA := (sA, [])]};
+        ipB := {[shB := (sB, mABm (state_get_m st))]}]}) →
+  (∀ (Hinv : anerisG (fair_model_to_model simple_fair_model) Σ),
+     ⊢ |={⊤}=>
+     unallocated A -∗
+     ([∗ set] a ∈ A, a ⤳[bool_decide (a ∈ obs_send_sas),
+                         bool_decide (a ∈ obs_rec_sas)] (∅, ∅)) -∗
+     live_roles_frag_own (simple_live_roles st ∖ config_roles) -∗
+     dead_roles_frag_own ((all_roles ∖ simple_live_roles st) ∖ config_roles) -∗
+     ([∗ set] i ∈ IPs, free_ip i) -∗
+     is_node ip -∗
+     ([∗ set] lbl ∈ lbls, alloc_evs lbl []) -∗
+     ([∗ set] sa ∈ obs_send_sas, sendon_evs sa []) -∗
+     ([∗ set] sa ∈ obs_rec_sas, receiveon_evs sa []) -∗
+     observed_send obs_send_sas -∗
+     observed_receive obs_rec_sas ={⊤}=∗
+     wptp s es (map (λ _ _, True) es) ∗
+     always_holds s valid_state_evolution_fairness (es, σ) st) ->
+  obs_send_sas ⊆ A → obs_rec_sas ⊆ A →
+  ip ∉ IPs →
+  dom (state_ports_in_use σ) = IPs →
+  (∀ ip, ip ∈ IPs → state_ports_in_use σ !! ip = Some ∅) →
+  (∀ a, a ∈ A → ip_of_address a ∈ IPs) →
+  state_heaps σ = {[ip:=∅]} →
+  state_sockets σ = {[ip:=∅]} →
+  state_ms σ = ∅ →
+  continued_simulation valid_state_evolution_fairness
+                       (trace_singleton (es, σ))
+                       (trace_singleton st).
+Proof.
+  intros Hlen HmABn HmABm Hwp Hsendle Hrecvle Hipdom Hpiiu Hip Hfixdom Hste Hsce Hmse.
+  apply (wp_strong_adequacy_multiple aneris_lang (fair_model_to_model simple_fair_model) Σ s);
+    [done| |].
+  { apply rel_finitary_valid_state_evolution_fairness. }
+  iIntros (?) "".
+  iMod node_gnames_auth_init as (γmp) "Hmp".
+  iMod saved_si_init as (γsi) "[Hsi Hsi']".
+  iMod (unallocated_init (to_singletons A)) as (γsif)
+    "[Hunallocated_auth Hunallocated]".
+  iMod (free_ips_init IPs) as (γips) "[HIPsCtx HIPs]".
+  iMod free_ports_auth_init as (γpiu) "HPiu".
+  iMod (allocated_address_groups_init (to_singletons obs_send_sas)) as
+      (γobserved_send) "#Hobserved_send".
+  iMod (allocated_address_groups_init (to_singletons obs_rec_sas)) as
+      (γobserved_receive) "#Hobserved_receive".
+  iMod (socket_address_group_ctx_init (to_singletons A)) as (γC) "Hauth";
+    [apply to_singletons_all_disjoint|].
+  iMod (socket_address_group_own_alloc_subseteq_pre _ (to_singletons A)
+                                                      (to_singletons A)
+         with "Hauth") as
+      "[Hauth HownA]"; [done|].
+  iDestruct (socket_address_group_own_big_sepS with "HownA") as "#HownAS".
+  iMod (messages_ctx_init (to_singletons A) _ _ _ _ with "HownAS Hobserved_send Hobserved_receive" ) as (γms) "[Hms HB]".
+  iMod (steps_init 1) as (γsteps) "[Hsteps _]".
+  iMod (roles_init (simple_live_roles st)) as (γlive) "[Hlivefull Hlivefrag]".
+  iMod (roles_init (all_roles ∖ simple_live_roles st))
+    as (γdead) "[Hdeadfull Hdeadfrag]".
+  iMod (alloc_evs_init lbls) as (γalevs) "[Halobctx Halobs]".
+  iMod (sendreceive_evs_init (to_singletons obs_send_sas)) as
+      (γsendevs) "[Hsendevsctx Hsendevs]".
+  iMod (sendreceive_evs_init (to_singletons obs_rec_sas)) as
+    (γreceiveevs) "[Hreceiveevsctx Hreceiveevs]".
+  (* NB: The model state is not used in the current state interpretation
+         and can be removed. *)
+  iMod (model_init (model_draft.Start:(fair_model_to_model simple_fair_model).(mstate))) as (γm) "[Hmfull Hmfrag]".
+  set (dg :=
+         {|
+           aneris_node_gnames_name := γmp;
+           aneris_si_name := γsi;
+           aneris_socket_address_group_name := γC;
+           aneris_unallocated_socket_address_groups_name := γsif;
+           aneris_freeips_name := γips;
+           aneris_freeports_name := γpiu;
+           aneris_messages_name := γms;
+           aneris_model_name := γm;
+           aneris_live_roles_name := γlive;
+           aneris_dead_roles_name := γdead;
+           aneris_steps_name := γsteps;
+           aneris_allocEVS_name := γalevs;
+           aneris_sendonEVS_name := γsendevs;
+           aneris_receiveonEVS_name := γreceiveevs;
+           aneris_observed_send_name := γobserved_send;
+           aneris_observed_recv_name := γobserved_receive;
+         |}).
+  iMod (Hwp dg) as "Hwp".
+  iMod (node_ctx_init ∅ ∅) as (γn) "[Hh Hs]".
+  iMod (node_gnames_alloc γn _ ip with "[$]") as "[Hmp #Hγn]"; [done|].
+  iAssert (is_node ip) as "Hn".
+  { iExists _. eauto. }
+  iExists (λ ex atr,
+      (⌜simple_valid_state_evolution ex atr⌝ ∗
+       aneris_events_state_interp ex ∗
+       aneris_state_interp
+         (trace_last ex).2
+         (trace_messages_history ex) ∗
+       thread_live_roles_interp (trace_last ex).1 (trace_last atr) ∗
+       steps_auth (trace_length ex)))%I.
+  iExists (map (λ _ _, True)%I es), (λ _ _, True)%I.
+  (* iExists (λ _, dead_role_frag_own A_role ∗ *)
+  (*               dead_role_frag_own B_role)%I, (λ _ _, True)%I. *)
+  iSplitR; [by iApply config_wp_correct|].
+   iMod (socket_address_group_own_alloc_subseteq_pre _ (to_singletons A) (to_singletons obs_send_sas) with "Hauth")
+    as "[Hauth Hown_send]".
+   { intros x Hin. eapply elem_of_to_singletons. set_solver. }
+  iDestruct (socket_address_group_own_big_sepS with "Hown_send") as "Hown_send".
+  iMod (socket_address_group_own_alloc_subseteq_pre _ (to_singletons A) (to_singletons obs_rec_sas) with "Hauth")
+    as "[Hauth Hown_recv]".
+  { intros x Hin. eapply elem_of_to_singletons. set_solver. }
+  iAssert (live_roles_frag_own ((simple_live_roles st) ∖ config_roles) ∗
+           live_roles_frag_own ((simple_live_roles st) ∩ config_roles))%I with
+            "[Hlivefrag]" as "[Hlivefrag Hlivefrag_cfg]".
+  { iApply live_roles_own_split; [set_solver|].
+    by rewrite -gset_union_difference_intersection_L. }
+  iAssert (dead_roles_frag_own ((all_roles ∖ simple_live_roles st) ∖ config_roles) ∗
+           dead_roles_frag_own ((all_roles ∖ simple_live_roles st) ∩ config_roles))%I with
+            "[Hdeadfrag]" as "[Hdeadfrag Hdeadfrag_cfg]".
+  { iApply dead_roles_own_split; [set_solver|].
+    by rewrite -gset_union_difference_intersection_L. }
+  iDestruct (socket_address_group_own_big_sepS with "Hown_recv") as "Hown_recv".
+  iDestruct ("Hwp" with "Hunallocated [HB] Hlivefrag Hdeadfrag HIPs Hn Halobs
+            [Hsendevs Hown_send] [Hreceiveevs Hown_recv]
+            Hobserved_send Hobserved_receive") as ">[Hwp H]".
+  { iApply (big_sepS_to_singletons with "[] HB").
+    iIntros "!>" (x) "Hx".
+    iDestruct "Hx" as (As Ar) "(?&?&[%%]&?&?)".
+    iFrame. simpl. iSplitL; [|done].
+    iExists _, _. iFrame.
+    iPureIntro.
+    rewrite H H0. rewrite !bool_decide_eq_true. set_solver. }
+  { iApply big_sepS_sep.
+    iSplitL "Hown_send".
+    - iApply (big_sepS_to_singletons with "[] Hown_send"); by eauto.
+    - iApply (big_sepS_to_singletons with "[] Hsendevs"); by eauto. }
+  { iApply big_sepS_sep.
+    iSplitL "Hown_recv".
+    - iApply (big_sepS_to_singletons with "[] Hown_recv"); by eauto.
+    - iApply (big_sepS_to_singletons with "[] Hreceiveevs"); by eauto. }
+  iMod (socket_address_group_own_alloc_subseteq_pre _ (to_singletons A)
+                                                    (to_singletons (obs_send_sas ∪ obs_rec_sas)) with "Hauth")
+    as "[Hauth Hown_send_recv]"; [by set_solver|].
+  rewrite to_singletons_union.
+  iPoseProof (aneris_events_state_interp_init with "[$] [$] [$] [$] [$] [$]") as "$".
+  iMod (socket_address_group_own_alloc_subseteq_pre _ (to_singletons A)
+                                                    (to_singletons A) with "Hauth")
+    as "[Hauth Hown]"; [by set_solver|].
+  iPoseProof (@aneris_state_interp_init _ _ dg IPs
+               with "Hmp [//] Hh Hs Hms [$Hauth $Hown] Hunallocated_auth Hsi HIPsCtx HPiu") as "Hinterp"; eauto.
+  { intros sag sa Hsag Hsa.
+    apply Hfixdom.
+    assert (is_singleton sag) as [sa' ->]; [by eapply elem_of_to_singletons_inv|].
+    apply elem_of_to_singletons in Hsag.
+    set_solver. }
+  { iPureIntro. apply to_singletons_fmap. intros x.
+    rewrite /is_ne. set_solver. }
+  iModIntro.
+  iFrame "Hwp".
+  iSplitR "H".
+  { iSplitR.
+    { iPureIntro. split; [constructor|done]. }
+    iFrame "Hsteps".
+    (* TODO: Change definition in state interp *)
+    replace ((all_roles ∖ simple_live_roles st) ∩ config_roles) with
+      (config_roles ∖ simple_live_roles st) by set_solver.
+    rewrite /= Hmse /= dom_empty_L. by iFrame. }
+  iIntros (ex atr c Hvalex Hstartex Hstartatr Hendex Hcontr Hstuck) "Hsi Hposts".
+  iDestruct "Hsi" as "(%Hvalid&_)".
+  iApply fupd_mask_intro; [set_solver|].
+  iIntros "_".
+  iPureIntro.
+  by destruct Hvalid as (Htrace&Hlabels&_).
+Qed.
 
 Theorem strong_simulation_adequacy Σ
     `{!anerisPreG (fair_model_to_model simple_fair_model) Σ}
@@ -156,13 +337,13 @@ Proof.
   iAssert (live_roles_frag_own ((simple_live_roles st) ∖ config_roles) ∗
            live_roles_frag_own ((simple_live_roles st) ∩ config_roles))%I with
             "[Hlivefrag]" as "[Hlivefrag Hlivefrag_cfg]".
-  { iApply live_roles_own_split; [set_solver|]. 
+  { iApply live_roles_own_split; [set_solver|].
     by rewrite -gset_union_difference_intersection_L. }
   iAssert (dead_roles_frag_own ((all_roles ∖ simple_live_roles st) ∖ config_roles) ∗
            dead_roles_frag_own ((all_roles ∖ simple_live_roles st) ∩ config_roles))%I with
             "[Hdeadfrag]" as "[Hdeadfrag Hdeadfrag_cfg]".
   { iApply dead_roles_own_split; [set_solver|].
-    by rewrite -gset_union_difference_intersection_L. }  
+    by rewrite -gset_union_difference_intersection_L. }
   iDestruct (socket_address_group_own_big_sepS with "Hown_recv") as "Hown_recv".
   iDestruct ("Hwp" with "Hunallocated [HB] Hlivefrag Hdeadfrag HIPs Hn Halobs
             [Hsendevs Hown_send] [Hreceiveevs Hown_recv]
@@ -192,14 +373,14 @@ Proof.
     as "[Hauth Hown]"; [by set_solver|].
   iPoseProof (@aneris_state_interp_init _ _ dg IPs
                with "Hmp [//] Hh Hs Hms [$Hauth $Hown] Hunallocated_auth Hsi HIPsCtx HPiu") as "Hinterp"; eauto.
-  { intros sag sa Hsag Hsa. 
+  { intros sag sa Hsag Hsa.
     apply Hfixdom.
     assert (is_singleton sag) as [sa' ->]; [by eapply elem_of_to_singletons_inv|].
     apply elem_of_to_singletons in Hsag.
     set_solver. }
   { iPureIntro. apply to_singletons_fmap. intros x.
     rewrite /is_ne. set_solver. }
-  iModIntro.  
+  iModIntro.
   iFrame "Hwp".
   iSplitR "H".
   { iSplitR.
@@ -239,30 +420,190 @@ Definition fair_network_ex (extr : extrace aneris_lang) :=
 Definition fair_ex (extr : extrace aneris_lang) :=
   (∀ ζ, fair_scheduling_ex ζ extr) ∧ fair_network_ex extr.
 
-Definition traces_match (extr : extrace aneris_lang)
-           (mtr : mtrace simple_fair_model) := True.
+(* Correspondence between live configurations and model states *)
+Definition live_tids (c : cfg aneris_lang) (δ : simple_state) : Prop :=
+  ∀ ζ (ℓ:fmrole simple_fair_model),
+  labels_match ζ ℓ → (role_enabled_model ℓ δ ↔ live_ex_label ζ c).
 
+Definition exmtr_traces_match : extrace aneris_lang → mtrace simple_fair_model → Prop :=
+  traces_match labels_match live_tids language.locale_step simple_trans.
+
+(* TODO: Derive from `valid_state_evolution_fairness` *)
+(* OBS: Need to bump definition to include `live_tids` *)
 Lemma continued_simulation_traces_match extr mtr :
   continued_simulation valid_state_evolution_fairness
                        {tr[trfirst extr]} {tr[trfirst mtr]} →
-  traces_match extr mtr.
+  exmtr_traces_match extr mtr.
 Proof. Admitted.
 
 Lemma traces_match_valid_preserved extr mtr :
-  traces_match extr mtr → mtrace_valid mtr.
-Proof. Admitted.
+  exmtr_traces_match extr mtr → mtrace_valid mtr.
+Proof.
+  revert extr mtr. pcofix CH. intros extr mtr Hmatch.
+  inversion Hmatch; first by (pfold; constructor).
+  pfold.
+  constructor =>//.
+  specialize (CH _ _ H3).
+  right. done.
+Qed.
 
 Lemma continued_simulation_valid_preserved
         (extr : extrace aneris_lang) (mtr : mtrace simple_fair_model) :
   continued_simulation valid_state_evolution_fairness
     ({tr[trfirst extr]}) ({tr[trfirst mtr]}) →
   mtrace_valid mtr.
-Proof. Admitted.
+Proof.
+  intros ?%continued_simulation_traces_match.
+  by eapply traces_match_valid_preserved.
+Qed.
+
+(* TODO: Move the lemmas relalted to general `traces_match` *)
+Definition flip_impl {A B} (R : A → B → Prop) : Prop :=
+  ∀ a b, R a b ↔ flip R b a.
+
+Lemma traces_match_flip {S1 S2 L1 L2}
+      (Rℓ: L1 -> L2 -> Prop) (Rs: S1 -> S2 -> Prop)
+      (trans1: S1 -> L1 -> S1 -> Prop)
+      (trans2: S2 -> L2 -> S2 -> Prop)
+      tr1 tr2 :
+  flip_impl Rℓ → flip_impl Rs →
+  traces_match Rℓ Rs trans1 trans2 tr1 tr2 ↔
+  traces_match (flip Rℓ) (flip Rs) trans2 trans1 tr2 tr1.
+Proof.
+  split.
+  - revert tr1 tr2. cofix CH.
+    intros tr1 tr2 Hmatch. inversion Hmatch; simplify_eq.
+    { by constructor. }
+    constructor; [done..|].
+    by apply CH.
+  - revert tr1 tr2. cofix CH.
+    intros tr1 tr2 Hmatch. inversion Hmatch; simplify_eq.
+    { by constructor. }
+    constructor; [done..|].
+    by apply CH.
+Qed.
+
+Lemma traces_match_traces_implies {S1 S2 L1 L2}
+      (Rℓ: L1 -> L2 -> Prop) (Rs: S1 -> S2 -> Prop)
+      (trans1: S1 -> L1 -> S1 -> Prop)
+      (trans2: S2 -> L2 -> S2 -> Prop)
+      (P1 Q1 : S1 → option L1 → Prop)
+      (P2 Q2 : S2 → option L2 → Prop)
+      tr1 tr2 :
+  flip_impl Rℓ → flip_impl Rs →
+  traces_match Rℓ Rs trans1 trans2 tr1 tr2 →
+  (∀ s1 s2 oℓ1 oℓ2, Rs s1 s2 →
+                    match oℓ1, oℓ2 with
+                    | Some ℓ1, Some ℓ2 => Rℓ ℓ1 ℓ2
+                    | None, None => True
+                    | _, _ => False
+                    end →
+                    P2 s2 oℓ2 → P1 s1 oℓ1) →
+  (∀ s1 s2 oℓ1 oℓ2, Rs s1 s2 →
+                    match oℓ1, oℓ2 with
+                    | Some ℓ1, Some ℓ2 => Rℓ ℓ1 ℓ2
+                    | None, None => True
+                    | _, _ => False
+                    end → Q1 s1 oℓ1 → Q2 s2 oℓ2) →
+  trace_implies P1 Q1 tr1 → trace_implies P2 Q2 tr2.
+Proof.
+  intros HRℓ HRs Hmatch HP HQ Htr1.
+  intros n Hpred_at.
+  rewrite /pred_at in Hpred_at.
+  assert (traces_match (flip Rℓ)
+                       (flip Rs)
+                       trans2 trans1
+                       tr2 tr1) as Hmatch'.
+  { by rewrite -traces_match_flip. }
+  destruct (after n tr2) as [tr2'|] eqn:Htr2eq; [|done].
+  eapply (traces_match_after) in Hmatch as (tr1' & Htr1eq & Hmatch); [|done].
+  specialize (Htr1 n).
+  rewrite {1}/pred_at in Htr1.
+  rewrite Htr1eq in Htr1.
+  destruct tr1' as [|s ℓ tr']; inversion Hmatch; simplify_eq; try by done.
+  - assert (P1 s None) as HP1 by by eapply (HP _ _ _ None).
+    destruct (Htr1 HP1) as [m Htr1'].
+    exists m. rewrite pred_at_sum. rewrite pred_at_sum in Htr1'.
+    destruct (after n tr1) as [tr1'|] eqn:Htr1eq'; [|done].
+    eapply (traces_match_after) in Hmatch' as (tr2' & Htr2eq' & Hmatch'); [|done].
+    rewrite Htr2eq'.
+    rewrite /pred_at.
+    rewrite /pred_at in Htr1'.
+    destruct (after m tr1') as [tr1''|] eqn:Htr1eq''; [|done].
+    eapply (traces_match_after) in Hmatch' as (tr2'' & Htr2eq'' & Hmatch''); [|done].
+    rewrite Htr2eq''.
+    destruct tr1''; inversion Hmatch''; simplify_eq; try by done.
+    + by eapply (HQ _ _ None None).
+    + by (eapply (HQ _ _ (Some _) _)).
+  - assert (P1 s (Some ℓ)) as HP1 by by (eapply (HP _ _ _ (Some _))).
+    destruct (Htr1 HP1) as [m Htr1'].
+    exists m. rewrite pred_at_sum. rewrite pred_at_sum in Htr1'.
+    destruct (after n tr1) as [tr1'|] eqn:Htr1eq'; [|done].
+    eapply (traces_match_after) in Hmatch' as (tr2' & Htr2eq' & Hmatch'); [|done].
+    rewrite Htr2eq'.
+    rewrite /pred_at.
+    rewrite /pred_at in Htr1'.
+    destruct (after m tr1') as [tr1''|] eqn:Htr1eq''; [|done].
+    eapply (traces_match_after) in Hmatch' as (tr2'' & Htr2eq'' & Hmatch''); [|done].
+    rewrite Htr2eq''.
+    destruct tr1''; inversion Hmatch''; simplify_eq; try by done.
+    + by eapply (HQ _ _ None None).
+    + by (eapply (HQ _ _ (Some _) _)).
+Qed.
+
+(* TODO: Move this *)
+Definition simple_label_locale (ℓ : simple_role) : ex_label aneris_lang :=
+  match ℓ with
+  | A_role => inl ("0.0.0.0",0)
+  | B_role => inl ("0.0.0.1",0)
+  | Ndeliver => inr DeliverLabel
+  | Ndrop => inr DropLabel
+  | Ndup => inr DuplicateLabel
+  end.
 
 Lemma traces_match_fairness_preserved extr mtr :
-  traces_match extr mtr →
+  exmtr_traces_match extr mtr →
   fair_ex extr → mtrace_fair mtr.
-Proof. Admitted.
+Proof.
+  rewrite /fair_ex /mtrace_fair.
+  intros Hmatch [Hfairex_scheduling Hfairex_network].
+  assert (mtrace_valid mtr) as Hvalid.
+  { by eapply traces_match_valid_preserved. }
+  split.
+  - intros ℓ.
+    assert (∃ ζ, labels_match ζ ℓ) as [ζ Hlabel].
+    { exists (simple_label_locale ℓ). destruct ℓ; done. }
+    specialize (Hfairex_scheduling ζ).
+    eapply traces_match_traces_implies; [by split|by split|done| | |done].
+    + intros s1 s2 oℓ1 oℓ2 Hlive HRℓ Henabled.
+      simpl in *. simplify_eq.
+      apply Hlive in Hlabel.
+      by apply Hlabel.
+    + intros s1 s2 oℓ1 oℓ2 Hlive HRℓ [Henabled|Henabled]; simpl in *.
+      * left. intros Henabled'. apply Henabled.
+        apply Hlive in Hlabel.
+        by apply Hlabel.
+      * right.
+        rewrite Henabled in HRℓ. destruct oℓ2; [|done].
+        simplify_eq. rewrite Hlabel. rewrite HRℓ. done.
+  - intros n. rewrite /pred_at.
+    specialize (Hfairex_network n). rewrite /pred_at in Hfairex_network.
+    destruct (after n extr) eqn:Heqn; [|done].
+    apply traces_match_flip in Hmatch; [|done..].
+    eapply (traces_match_after) in Hmatch as (mtr' & Hmtreq & Hmatch); [|done].
+    rewrite Hmtreq.
+    destruct t; inversion Hmatch; simplify_eq; [done|].
+    destruct Hfairex_network as [Hdup Hdrop].
+    split.
+    + rewrite H2.
+      intros Heq. apply Hdup. simplify_eq.
+      admit. (* Weird matching inversion stuff. *)
+    + rewrite H2. intros Heq.
+      apply Hdrop.
+      simplify_eq.
+      rewrite /locale_simple_label in Heq.
+      admit. (* Weird matching inversion stuff. *)
+Admitted.
 
 Theorem continued_simulation_fairness_preserved
         (extr : extrace aneris_lang) (mtr : mtrace simple_fair_model) :
@@ -275,7 +616,7 @@ Proof.
 Qed.
 
 Lemma traces_match_termination_preserved extr mtr :
-  traces_match extr mtr →
+  exmtr_traces_match extr mtr →
   terminating_trace mtr →
   terminating_trace extr.
 Proof. Admitted.
