trillium/program_logic/adequacy.v
@@ -803,6 +803,272 @@ Lemma fupd_to_bupd_soundness_no_lc' `{!invGpreS Σ} (Q : iProp Σ) `{!Plain Q} :
   (∀ `{Hinv: !invGS_gen HasNoLc Σ}, fupd_to_bupd ⊤ -∗ Q) → ⊢ Q.
 Proof. by iIntros; iApply bupd_plain; iApply fupd_to_bupd_soundness_no_lc. Qed.
 
+Theorem wp_strong_adequacy_multiple_helper Σ Λ M `{!invGpreS Σ}
+        (s: stuckness) (ξ : execution_trace Λ → auxiliary_trace M → Prop)
+        es σ δ:
+  length es ≥ 1 →
+  (∀ `{Hinv : !invGS_gen HasNoLc Σ},
+    ⊢ |={⊤}=> ∃
+         (stateI : execution_trace Λ → auxiliary_trace M → iProp Σ)
+         (trace_inv : execution_trace Λ → auxiliary_trace M → iProp Σ)
+         (Φs : list (val Λ → iProp Σ))
+         (fork_post : locale Λ → val Λ → iProp Σ),
+       let _ : irisG Λ M Σ := IrisG _ _ _ Hinv stateI fork_post in
+       (* ⌜length Φs = length es⌝ ∗ *)
+       config_wp ∗
+       stateI (trace_singleton (es, σ)) (trace_singleton δ) ∗
+       wptp s es Φs ∗
+       (∀ (ex : execution_trace Λ) (atr : auxiliary_trace M) c,
+         ⌜valid_system_trace ex atr⌝ -∗
+         ⌜trace_starts_in ex (es, σ)⌝ -∗
+         ⌜trace_starts_in atr δ⌝ -∗
+         ⌜trace_ends_in ex c⌝ -∗
+         ⌜∀ ex' atr' oζ ℓ, trace_contract ex oζ ex' →
+                           trace_contract atr ℓ atr' → ξ ex' atr'⌝ -∗
+         ⌜∀ e2, s = NotStuck → e2 ∈ c.1 → not_stuck e2 c.2⌝ -∗
+         stateI ex atr -∗
+         posts_of c.1 (Φs ++ (map (λ '(tnew, e), fork_post (locale_of tnew e)) (prefixes_from es (drop (length es) c.1)))) -∗
+         □ (stateI ex atr ∗
+             (∀ ex' atr' oζ ℓ, ⌜trace_contract ex oζ ex'⌝ → ⌜trace_contract atr ℓ atr'⌝ → trace_inv ex' atr')
+            ={⊤}=∗ stateI ex atr ∗ trace_inv ex atr) ∗
+         ((∀ ex' atr' oζ ℓ,
+              ⌜trace_contract ex oζ ex'⌝ → ⌜trace_contract atr ℓ atr'⌝ → trace_inv ex' atr')
+          ={⊤, ∅}=∗ ⌜ξ ex atr⌝))) →
+  ⊢ Gsim Σ M s ξ (trace_singleton (es, σ)) (trace_singleton δ).
+Proof.
+  intros Hes Hwp.
+  apply extract_except_0.
+  iApply fupd_to_bupd_soundness_no_lc'.
+  iIntros (Hinv) "HFtB".
+  rewrite fupd_to_bupd_unfold /fupd_to_bupd_aux.
+  iApply bupd_plain.
+  iApply "HFtB".
+  iPoseProof (Hwp Hinv) as "Hwp".
+  iMod "Hwp" as (stateI trace_inv Φs fork_post) "(#config_wp & HSI & Hwp & Hstep)".
+  clear Hwp.
+  set (IrisG Λ M Σ Hinv stateI fork_post).
+  iAssert (∃ ex atr c1 δ1,
+              ⌜trace_singleton (es, σ) = ex⌝ ∗
+              ⌜trace_singleton δ = atr⌝ ∗
+              ⌜(es, σ) = c1⌝ ∗
+              ⌜δ = δ1⌝ ∗
+              ⌜length c1.1 ≥ 1⌝ ∗
+              stateI ex atr ∗
+              (∀ ex' atr' oζ ℓ,
+                  ⌜trace_contract ex oζ ex'⌝ → ⌜trace_contract atr ℓ atr'⌝ → trace_inv ex' atr') ∗
+              wptp s c1.1 (Φs ++ map (λ '(tnew, e), fork_post (locale_of tnew e)) (prefixes_from es (drop (length es) c1.1))))%I
+    with "[HSI Hwp]" as "Hex".
+  { iExists (trace_singleton (es, σ)), (trace_singleton δ), (es, σ), δ; simpl.
+    rewrite drop_ge; [|lia]. rewrite right_id.
+    iFrame.
+    repeat (iSplit; first by auto).
+    iIntros (???? ?%not_trace_contract_singleton); done. }
+  iDestruct "Hex" as (ex atr c1 δ1 Hexsing Hatrsing Hc1 Hδ1 Hlen) "(HSI & HTI & Htp)".
+  assert
+    (valid_system_trace ex atr ∧
+     trace_starts_in ex (es, σ) ∧
+     trace_ends_in ex c1 ∧
+     trace_starts_in atr δ ∧
+     (∀ ex' atr' oζ ℓ,
+         trace_contract ex oζ ex' → trace_contract atr ℓ atr' → ξ ex' atr'))
+    as Hextras.
+  { rewrite -Hexsing -Hatrsing -Hc1.
+    split; first apply valid_system_trace_singletons.
+    repeat (split; first done).
+    intros ? ? ? ? ? ?%not_trace_contract_singleton; done. }
+  clear Hc1 Hδ1.
+  rewrite Hexsing Hatrsing; clear Hexsing Hatrsing.
+  iLöb as "IH" forall (ex atr c1 Hextras Hlen) "HSI HTI Htp".
+  destruct Hextras as (Hv & Hex & Hc1 & Hatr & Hξ).
+  rewrite {2}/Gsim (fixpoint_unfold (Gsim_pre _ _ _ _) _ _).
+  destruct c1 as [tp σ1'].
+  assert (valid_exec ex) as Hexv.
+  { by eapply valid_system_trace_valid_exec_trace. }
+  iPoseProof (wptp_not_stuck _ _ _ _ _ _ [] with "[$HSI] Htp") as "Htp";
+    [apply locales_equiv_refl|done|by list_simplifier|].
+  iMod ("Htp") as "(HSI & Htp & %Hnstk)".
+  rewrite (last_eq_trace_ends_in _ (tp, σ1')) in Hnstk; last done.
+  iPoseProof (wptp_of_val_post with "Htp") as "Htp".
+  iMod ("Htp") as "(Hpost & Hback)".
+  iAssert (|={⊤}=> ▷ ⌜ξ ex atr⌝ ∗ (_ ∗ _ ∗ _ ∗ _))%I with "[Hstep HTI HSI Hpost]"
+    as ">[Hξ (HSI & Hpost & HTI & Hstep)]".
+  { iCombine "HTI" "Hstep" as "HS".
+    iCombine "Hpost" "HS" as "HS".
+    iCombine "HSI" "HS" as "HS".
+    iApply fupd_plain_keep_l; iSplitR; [|iExact "HS"].
+    iIntros "(HSI & Hpost & HTI & Hstep)".
+    iDestruct ("Hstep" with "[] [] [] [] [] [] HSI Hpost") as "[_ Hξ]"; auto.
+    iApply fupd_plain_mask.
+    iMod ("Hξ" with "HTI") as "%"; auto. }
+  iAssert (□ (stateI ex atr -∗
+             (∀ ex' atr' oζ ℓ,
+                 ⌜trace_contract ex oζ ex'⌝ → ⌜trace_contract atr ℓ atr'⌝ → trace_inv ex' atr')
+                 ={⊤}=∗ stateI ex atr ∗ trace_inv ex atr))%I as "#HTIextend".
+  { iDestruct ("Hstep" with "[] [] [] [] [] [] HSI Hpost") as "[#Hext _]"; auto.
+    iModIntro.
+    iIntros "HSI HTI".
+    iApply ("Hext" with "[$HSI $HTI]"). }
+  iMod ("HTIextend" with "HSI HTI") as "[HSI HTI]".
+  iDestruct ("Hback" with "Hpost") as "Htp".
+  iModIntro.
+  iIntros "HFtB".
+  iNext; iSplit; first done.
+  iDestruct "Hξ" as %Hξ'.
+  iIntros (c oζ c' Hc Hstep).
+  pose proof (trace_ends_in_inj ex c (tp, σ1') Hc Hc1); simplify_eq.
+  iPoseProof (take_step with "config_wp HSI Htp") as "Hstp"; [done|done|done|].
+  assert (∃ n, n = trace_length ex) as [n Hn] by eauto.
+  rewrite -Hn.
+  clear Hn.
+  rewrite -> fupd_to_bupd_unfold; rewrite /fupd_to_bupd_aux.
+  iApply except_0_later.
+  iApply bupd_plain.
+  iApply "HFtB".
+  iMod "Hstp"; simpl.
+  iMod "Hstp".
+  iModIntro.
+  iIntros "HFtB".
+  rewrite (fupd_to_bupd_unfold (∅ : coPset)); rewrite /fupd_to_bupd_aux.
+  iNext.
+  iApply except_0_later.
+  iApply bupd_plain.
+  iApply "HFtB".
+  iMod "Hstp".
+  iModIntro.
+  iIntros "HFtB".
+  iInduction n as [|n] "IHlen"; simpl; last first.
+  { rewrite (fupd_to_bupd_unfold (∅ : coPset)); rewrite /fupd_to_bupd_aux.
+    iApply except_0_later.
+    iApply bupd_plain.
+    iApply "HFtB".
+    iMod "Hstp".
+    iModIntro.
+    iIntros "HFtB".
+    rewrite (fupd_to_bupd_unfold (∅ : coPset)); rewrite /fupd_to_bupd_aux.
+    iNext.
+    iApply except_0_later.
+    iApply bupd_plain.
+    iApply "HFtB".
+    iMod "Hstp".
+    iModIntro.
+    iIntros "HFtB".
+    rewrite (fupd_to_bupd_unfold (∅ : coPset)); rewrite /fupd_to_bupd_aux.
+    iApply ("IHlen" with "Hstep HTI Hstp"); done. }
+  rewrite (fupd_to_bupd_unfold (∅ : coPset)); rewrite /fupd_to_bupd_aux.
+  iApply except_0_later.
+  iApply bupd_plain.
+  iApply "HFtB".
+  iMod "Hstp" as "(% & H)".
+  iModIntro.
+  iIntros "HFtB".
+  iDestruct "H" as (δ'' ℓ) "(HSI & Hpost & Hback)"; simpl in *.
+  iSpecialize ("Hback" with "Hpost").
+  assert (Hlocales: map (λ '(tnew, e), weakestpre.fork_post (locale_of tnew e))
+                    (prefixes_from es (drop (length es) tp)) ++
+                  map (λ '(tnew, e), weakestpre.fork_post (locale_of tnew e))
+                  (prefixes_from tp (drop (length tp) c'.1))
+         = map (λ '(tnew, e), weakestpre.fork_post (locale_of tnew e))
+                    (prefixes_from es (drop (length es) c'.1)) ).
+  { pose proof (locale_valid_exec _ _ _ _ _ Hexv Hex Hc) as Hequivex.
+    induction es as [|e1 es IHes].
+    { simpl in *. lia. }
+    destruct c'.1 as [|e3 tp3_rest] eqn:Heq.
+    { exfalso. pose proof (step_tp_length _ _ _ Hstep). rewrite ->Heq in *. simpl in *. lia. }
+    destruct tp as [|e2 tp2_rest] eqn:Heq'.
+    { simpl in Hlen; lia. }
+    change fork_post with weakestpre.fork_post.
+    assert (locale_of [] e1 = locale_of [] e2); first by inversion Hequivex.
+    change 1 with (length [e1]).
+    (* TODO: You are here *)
+Admitted.
+
+(*     assert (∀ A (x : A) xs, x :: xs = [x] ++ xs) as Happ_cons by set_solver. *)
+(*     simpl. *)
+(*     rewrite (Happ_cons _ e1). *)
+(*     rewrite (Happ_cons _ e2). *)
+(*     rewrite !(newposts_locales_equiv [e1] [e2]). *)
+
+(*     rewrite !(newposts_locales_equiv es tp). *)
+
+
+
+(*     (* destruct tp as [|e2 tp2_rest] eqn:Heq'. *) *)
+(*     (* { simpl in Hlen; lia. } *) *)
+(*     change fork_post with weakestpre.fork_post. *)
+(*     (* assert (locale_of [] e1 = locale_of [] e2); first by inversion Hequivex. *) *)
+(*     (* change 1 with (length [e1]). *) *)
+(*     rewrite !(newposts_locales_equiv es tp). *)
+(*     2: { constructor. *)
+
+(*     (* TODO: You are here *) *)
+
+(*     [| by constructor =>// | by constructor =>//]. *)
+(*     rewrite ![drop _ _]/=. *)
+(*     rewrite drop_0. *)
+(*     assert (Hequiv: locales_equiv (e2 :: tp2_rest) (take (length (e2 :: tp2_rest)) (e3 :: tp3_rest))). *)
+(*     { pose proof (locale_step_equiv _ _ _ Hstep) as Hequiv. *)
+(*       rewrite Heq // in Hequiv. } *)
+(*     assert (Hequiv_from: locales_equiv_from [e2] [e3] tp2_rest (take (length tp2_rest) tp3_rest)). *)
+(*     { change [e2] with ([] ++ [e2]). *)
+(*       change [e3] with ([] ++ [e3]). *)
+(*       change (e2 :: tp2_rest) with ([e2] ++ tp2_rest) in Hequiv. *)
+(*       rewrite [take _ _]/= in Hequiv. *)
+(*       change (e3 :: take (length tp2_rest) tp3_rest) with ([e3] ++ take (length tp2_rest) tp3_rest) in Hequiv. *)
+(*       assert (length tp2_rest = length (take (length tp2_rest) tp3_rest)) as Hlen'. *)
+(*       { rewrite take_length. pose proof (step_tp_length _ _ _ Hstep) as Hdec. *)
+(*         rewrite Heq /= in Hdec. lia. } *)
+(*       apply (locales_equiv_from_impl _ _ _ _ _ _ Hlen' Hequiv) =>//. } *)
+(*     erewrite forkposts_locales_equiv; last done. *)
+(*     assert (Hequiv_from': forall t, locales_equiv_from (e2 :: tp2_rest) (e3 :: take (length tp2_rest) tp3_rest) t t). *)
+(*     { intros t. by apply locales_from_equiv_refl. } *)
+(*     erewrite (forkposts_locales_equiv (e2 :: tp2_rest)); last first. *)
+(*     { eauto using Hequiv_from'. } *)
+(*     assert (Hequiv_from'': forall t, locales_equiv_from [e2] [e3] t t). *)
+(*     { intros t. apply locales_from_equiv_refl. constructor =>//. by inversion Hequiv. } *)
+(*     erewrite (forkposts_locales_equiv [e2]); last by eauto. *)
+(*     rewrite -map_app -prefixes_from_app take_drop. *)
+(*     rewrite [drop _ _]/= drop_0 //. } *)
+(*   iAssert (▷ ⌜ξ (ex :tr[oζ]: c') (atr :tr[ℓ]: δ'')⌝)%I as "#Hextend'". *)
+(*   { iDestruct ("Hstep" with "[] [] [] [] [] [] HSI") as "H"; [iPureIntro..|]. *)
+(*     - eapply valid_system_trace_extend; eauto. *)
+(*     - eapply trace_extend_starts_in; eauto. *)
+(*     - eapply trace_extend_starts_in; eauto. *)
+(*     - eapply trace_extend_ends_in; eauto. *)
+(*     - by intros ? ? ? ? [-> ->]%trace_contract_of_extend [-> ->]%trace_contract_of_extend. *)
+(*     - done. *)
+(*     - rewrite Hlocales. *)
+(*       iPoseProof (wptp_of_val_post with "Hback") as "Hback". *)
+(*       rewrite -> (fupd_to_bupd_unfold (⊤ : coPset)); rewrite /fupd_to_bupd_aux. *)
+(*       iApply except_0_later. *)
+(*       iApply bupd_plain. *)
+(*       iApply "HFtB". *)
+(*       iMod "Hback" as "(Hpost & Hwptp)". *)
+(*       iDestruct ("H" with "Hpost") as "[? Hξ]". *)
+(*       iMod ("Hξ" with "[HTI]") as "%". *)
+(*       + iIntros (? ? ? ? [-> ->]%trace_contract_of_extend *)
+(*                  [-> ->]%trace_contract_of_extend); done. *)
+(*       + iModIntro. *)
+(*         iIntros "HFtB"; done. } *)
+(*   iExists _, _. *)
+(*   rewrite -> (fupd_to_bupd_unfold (⊤ : coPset)); rewrite /fupd_to_bupd_aux. *)
+(*   iApply except_0_later. *)
+(*   iApply bupd_plain. *)
+(*   iApply "HFtB". *)
+(*   iMod ("IH" with "[] [] Hstep HSI [HTI] [Hback]") as "IH'". *)
+(*   - iPureIntro; split_and!. *)
+(*     + eapply valid_system_trace_extend; eauto. *)
+(*     + eapply trace_extend_starts_in; eauto. *)
+(*     + eapply trace_extend_ends_in; eauto. *)
+(*     + eapply trace_extend_starts_in; eauto. *)
+(*     + by intros ???? [-> ->]%trace_contract_of_extend *)
+(*                 [-> ->]%trace_contract_of_extend. *)
+(*   - iPureIntro. pose proof (step_tp_length _ _ _ Hstep). simpl in *. lia. *)
+(*   - iIntros (???? [-> ->]%trace_contract_of_extend *)
+(*                   [-> ->]%trace_contract_of_extend); done. *)
+(*   - rewrite Hlocales //. *)
+(*   - iModIntro. iIntros "HFtB". iNext. iApply "IH'"; done. *)
+(* Qed. *)
+
 Theorem wp_strong_adequacy_helper Σ Λ M `{!invGpreS Σ}
         (s: stuckness) (ξ : execution_trace Λ → auxiliary_trace M → Prop)
         e1 σ1 δ:
@@ -1071,13 +1337,13 @@ End finitary_lemma.
 
 (** We can extract the simulation correspondence in the meta-logic
     from a proof of the simulation correspondence in the object-logic. *)
-Theorem simulation_correspondence Λ M Σ `{!invGpreS Σ}
+Theorem simulation_correspondence_multiple Λ M Σ `{!invGpreS Σ}
         (s: stuckness)
         (ξ : execution_trace Λ → auxiliary_trace M → Prop)
-        e1 σ1 δ1 :
+        es σ δ :
   rel_finitary ξ →
-  (⊢ Gsim Σ M s ξ {tr[ ([e1], σ1) ]} {tr[ δ1 ]}) →
-  continued_simulation ξ {tr[ ([e1], σ1) ]} {tr[δ1]}.
+  (⊢ Gsim Σ M s ξ {tr[ (es, σ) ]} {tr[ δ ]}) →
+  continued_simulation ξ {tr[ (es, σ) ]} {tr[δ]}.
 Proof.
   intros Hsc Hwptp.
   exists (λ exatr, ⊢ Gsim Σ M s ξ exatr.1 exatr.2); split; first done.
@@ -1118,6 +1384,55 @@ Proof.
   intros [_ ?]; done.
 Qed.
 
+
+(** We can extract the simulation correspondence in the meta-logic
+    from a proof of the simulation correspondence in the object-logic. *)
+Theorem simulation_correspondence Λ M Σ `{!invGpreS Σ}
+        (s: stuckness)
+        (ξ : execution_trace Λ → auxiliary_trace M → Prop)
+        e1 σ1 δ1 :
+  rel_finitary ξ →
+  (⊢ Gsim Σ M s ξ {tr[ ([e1], σ1) ]} {tr[ δ1 ]}) →
+  continued_simulation ξ {tr[ ([e1], σ1) ]} {tr[δ1]}.
+Proof. by apply simulation_correspondence_multiple. Qed.
+
+Theorem wp_strong_adequacy_multiple_with_trace_inv Λ M Σ `{!invGpreS Σ}
+        (s: stuckness)
+        (ξ : execution_trace Λ → auxiliary_trace M → Prop)
+        es σ δ :
+  length es ≥ 1 →
+  rel_finitary ξ →
+  (∀ `{Hinv : !invGS_gen HasNoLc Σ},
+    ⊢ |={⊤}=> ∃
+         (stateI : execution_trace Λ → auxiliary_trace M → iProp Σ)
+         (trace_inv : execution_trace Λ → auxiliary_trace M → iProp Σ)
+         (Φs : list (val Λ → iProp Σ))
+         (fork_post : locale Λ → val Λ → iProp Σ),
+       let _ : irisG Λ M Σ := IrisG _ _ _ Hinv stateI fork_post in
+       config_wp ∗
+       stateI (trace_singleton (es, σ)) (trace_singleton δ) ∗
+       wptp s es Φs ∗
+       (∀ (ex : execution_trace Λ) (atr : auxiliary_trace M) (c : cfg Λ),
+         ⌜valid_system_trace ex atr⌝ -∗
+         ⌜trace_starts_in ex (es, σ)⌝ -∗
+         ⌜trace_starts_in atr δ⌝ -∗
+         ⌜trace_ends_in ex c⌝ -∗
+         ⌜∀ ex' atr' oζ ℓ, trace_contract ex oζ ex' → trace_contract atr ℓ atr' → ξ ex' atr'⌝ -∗
+         ⌜∀ e2, s = NotStuck → e2 ∈ c.1 → not_stuck e2 c.2⌝ -∗
+         stateI ex atr -∗
+         posts_of c.1 (Φs ++ (map (λ '(tnew, e), fork_post (locale_of tnew e)) (prefixes_from es (drop (length es) c.1)))) -∗
+         □ (stateI ex atr ∗
+             (∀ ex' atr' oζ ℓ, ⌜trace_contract ex oζ ex'⌝ → ⌜trace_contract atr ℓ atr'⌝ → trace_inv ex' atr')
+            ={⊤}=∗ stateI ex atr ∗ trace_inv ex atr) ∗
+         ((∀ ex' atr' oζ ℓ,
+              ⌜trace_contract ex oζ ex'⌝ → ⌜trace_contract atr ℓ atr'⌝ → trace_inv ex' atr')
+          ={⊤, ∅}=∗ ⌜ξ ex atr⌝))) →
+  continued_simulation ξ (trace_singleton (es, σ)) (trace_singleton δ).
+Proof.
+  intros Hlen Hsc Hwptp%wp_strong_adequacy_multiple_helper; [|by done..].
+  by eapply simulation_correspondence_multiple.
+Qed.
+
 Theorem wp_strong_adequacy_with_trace_inv Λ M Σ `{!invGpreS Σ}
         (s: stuckness)
         (ξ : execution_trace Λ → auxiliary_trace M → Prop)
@@ -1152,6 +1467,45 @@ Theorem wp_strong_adequacy_with_trace_inv Λ M Σ `{!invGpreS Σ}
 Proof.
   intros Hsc Hwptp%wp_strong_adequacy_helper; last done.
   by eapply simulation_correspondence.
+Qed.
+
+Theorem wp_strong_adequacy_multiple Λ M Σ `{!invGpreS Σ}
+        (s: stuckness)
+        (ξ : execution_trace Λ → auxiliary_trace M → Prop)
+        es σ δ :
+  length es ≥ 1 →
+  rel_finitary ξ →
+  (∀ `{Hinv : !invGS_gen HasNoLc Σ},
+    ⊢ |={⊤}=> ∃
+         (stateI : execution_trace Λ → auxiliary_trace M → iProp Σ)
+         (Φs : list (val Λ → iProp Σ))
+         (fork_post : locale Λ → val Λ → iProp Σ),
+       let _ : irisG Λ M Σ := IrisG _ _ _ Hinv stateI fork_post in
+       config_wp ∗
+       stateI (trace_singleton (es, σ)) (trace_singleton δ) ∗
+       wptp s es Φs ∗
+       (∀ (ex : execution_trace Λ) (atr : auxiliary_trace M) c,
+         ⌜valid_system_trace ex atr⌝ -∗
+         ⌜trace_starts_in ex (es, σ)⌝ -∗
+         ⌜trace_starts_in atr δ⌝ -∗
+         ⌜trace_ends_in ex c⌝ -∗
+         ⌜∀ ex' atr' oζ ℓ, trace_contract ex oζ ex' → trace_contract atr ℓ atr' → ξ ex' atr'⌝ -∗
+         ⌜∀ e2, s = NotStuck → e2 ∈ c.1 → not_stuck e2 c.2⌝ -∗
+         stateI ex atr -∗
+         posts_of c.1 (Φs ++ (map (λ '(tnew, e), fork_post (locale_of tnew e)) (prefixes_from es (drop (length es) c.1)))) -∗
+         |={⊤, ∅}=> ⌜ξ ex atr⌝)) ->
+  continued_simulation ξ (trace_singleton (es, σ)) (trace_singleton δ).
+Proof.
+  intros Hlen Hsc Hwptp.
+  eapply wp_strong_adequacy_multiple_with_trace_inv; [done|done|done|].
+  iIntros (Hinv) "".
+  iMod (Hwptp Hinv) as (stateI Φ fork_post) "(Hwpcfg & HSI & Hwp & Hstep)".
+  iModIntro.
+  iExists stateI, (λ _ _, True)%I, Φ, fork_post; iFrame "Hwpcfg HSI Hwp".
+  iIntros (ex atr c ? ? ? ? ? ?) "HSI Hposts".
+  iSplit; last first.
+  { iIntros "?". iApply ("Hstep" with "[] [] [] [] [] [] HSI"); eauto. }
+  iModIntro; iIntros "[$ ?]"; done.
 Qed.
 
 Theorem wp_strong_adequacy Λ M Σ `{!invGpreS Σ}
